cleanq/simpleq: more tries with autocorres
Signed-off-by: Reto Achermann <reto.achermann@inf.ethz.ch>

CleanQ/CleanQ_SimpleQ.thy
@@ -33,6 +33,14 @@ external_file "CleanQ_SimpleQ.c"
 install_C_file "CleanQ_SimpleQ.c"
 
 autocorres [
+
+  (* Name compatibility options *)
+  lifted_globals_field_prefix="c_glbl_",
+  lifted_globals_field_suffix="",
+  function_name_prefix="",
+  function_name_suffix="_c_fun",
+
+
   (* heap abstraction options *)
     
   (* no_heap_abs = FUNC_NAMES, *)
@@ -41,7 +49,7 @@ autocorres [
   (* force_heap_abs = FUNC_NAMES, *)
   (* Attempt _heap abstraction_  on the given list of functions *)
 
-  heap_abs_syntax,
+(*  heap_abs_syntax, *)
   (* Enable experimental heap abstraction syntactic sugar. *)
 
   (* skip_heap_abs *)
@@ -50,10 +58,10 @@ autocorres [
 
   (* word abstraction options *)
 
-  (* unsigned_word_abs = FUNC_NAMES, *)
+  unsigned_word_abs =   rb_can_deq rb_can_enq rb_enq rb_deq,
   (* Use _word abstraction_  on unsigned integers in the given functions. *)
 
-  (* no_signed_word_abs = FUNC_NAMES, *)
+  no_signed_word_abs = rb_can_enq rb_can_deq rb_enq rb_deq, 
   (* Disable signed  _word abstraction_ on the given list of functions. *)
 
   (* skip_word_abs, *)
@@ -61,10 +69,10 @@ autocorres [
 
 
   (* type strengthening options *)
-  (* ts_rules =  pure option nondet, *)
+  ts_rules =  pure option nondet, 
   (* Enable _type strengthening_ to the  following types. pure, option, gets nondet *)
 
-  (* ts_force RULE_NAME = FUNC_NAMES *)
+  ts_force nondet =  rb_can_deq rb_can_enq  rb_enq rb_deq,
   (* Force the given functions to be type-strengthened to the given type *)
 
 
@@ -99,21 +107,20 @@ autocorres [
 
   (* seL4 proof options *)
 
-  no_c_termination,
+  no_c_termination
   (*  Generate SIMPL wrappers and correspondence proofs *)
 
   (* c_locale = Name *)
   (*  Run in this locale, rather than the default locale *)
 
-
-  (* Name compatibility options *)
-  lifted_globals_field_prefix="c_glbl_",
-  lifted_globals_field_suffix="",
-  function_name_prefix="c_fun_",
-  function_name_suffix=""
 ] "CleanQ_SimpleQ.c"
 (* skip_word_abs *)
 
+
+
+record buffer =
+  base :: nat
+  length :: nat
 
 context CleanQ_SimpleQ begin
 
@@ -122,31 +129,140 @@ thm rb_init_body_def
 thm c_fun_rb_can_enq_def
 thm c_fun_rb_init_def
 thm rb_can_enq_body_def
-thm c_fun_rb_can_enq_def
+thm rb_can_enq_c_fun_def
+thm rb_can_enq_def
+
+
 thm rb_enq_body_def
 thm rb_can_deq_body_def
 
 thm rb_deq_body_def
 thm rb_can_enq_body_def
 term rb_C
+term buffer_C
+term head_C
 
 
-definition rb_C_to_CleanQ_RB :: "lifted_globals \<Rightarrow> rb_C ptr \<Rightarrow> nat  CleanQ_RB"
-  where "rb_C_to_CleanQ_RB s rb = \<lparr>  ring = \<lambda>x. 1,
-                                     head =  Word.unat (head_C (heap_rb_C s rb)), 
-                                     tail =  Word.unat (tail_C (heap_rb_C s rb)),
-                                     size =  Word.unat (size_C (heap_rb_C s rb)) \<rparr>"
+(* this one should be the pre-condition for the operation *)
+definition rb_valid_c :: " lifted_globals \<Rightarrow> rb_C ptr \<Rightarrow> bool"
+  where "rb_valid_c s rb \<longleftrightarrow> is_valid_rb_C s rb 
+                            \<and> unat (size_C (heap_rb_C s rb)) > 1 
+                            \<and> unat (head_C (heap_rb_C s rb)) < unat(size_C (heap_rb_C s rb))
+                            \<and> unat (tail_C (heap_rb_C s rb)) < unat(size_C (heap_rb_C s rb))"
 
-lemma foo:
-  "\<lbrace> \<lambda>s. True \<rbrace>
-   c_fun_rb_can_deq rb
-   \<lbrace> \<lambda> r s. r = 1 \<rbrace>!"
-  unfolding rb_can_deq_def apply(vcg)
 
-  unfolding  rb_C_to_CleanQ_RB_def rb_can_deq_def rb_empty_def
+definition
+  the_rb :: "lifted_globals \<Rightarrow> buffer_C ptr \<Rightarrow> nat \<Rightarrow> buffer"
+  where
+  "the_rb s b i =  \<lparr> base = unat (offset_C (heap_buffer_C s (b  +\<^sub>p i))),
+                     length = unat (length_C (heap_buffer_C s (b  +\<^sub>p i))) \<rparr>"
+
+definition rb_C_to_CleanQ_RB :: "lifted_globals \<Rightarrow> rb_C ptr \<Rightarrow> buffer  CleanQ_RB"
+  where "rb_C_to_CleanQ_RB s rb = \<lparr>  ring = \<lambda>i. the_rb s (ring_C (heap_rb_C s rb)) i,
+                                     head =  unat (head_C (heap_rb_C s rb)), 
+                                     tail =  unat (tail_C (heap_rb_C s rb)),
+                                     size =  unat (size_C (heap_rb_C s rb)) \<rparr>"
+
+lemma c_can_deq:
+  fixes rb :: "rb_C ptr"
+  shows 
+  "\<lbrace> \<lambda>s. rb_valid_c s rb  \<rbrace>
+   rb_can_deq_c_fun rb
+   \<lbrace> \<lambda> r s. r = (if rb_can_deq (rb_C_to_CleanQ_RB s rb) then 1 else 0) \<rbrace>!"
+  apply(subst rb_can_deq_c_fun_def)
+  apply(wp)
+  unfolding rb_can_deq_def rb_empty_def rb_C_to_CleanQ_RB_def rb_valid_c_def
+  by(auto)
+
+
+lemma foo1:
+ "unat (C :: 64 word) = ULONG_MAX \<Longrightarrow> (D :: 64 word) < C \<Longrightarrow> unat (D) < ULONG_MAX"
+  by(simp add: word_less_nat_alt)
+
+lemma foo2:
+ "unat (C :: 64 word) < ULONG_MAX \<Longrightarrow> (D :: 64 word) < C \<Longrightarrow> unat (D) < ULONG_MAX"
+  by(simp add: word_less_nat_alt)
+
+lemma foo3: "unat (C :: 64 word) \<le> ULONG_MAX \<Longrightarrow> (D :: 64 word) < C \<Longrightarrow> unat (D) < ULONG_MAX"
+  using foo1 foo2 PackedTypes.order_leE 
+  by blast
+
+lemma foo4:
+  "unat (C :: 64 word) \<le> ULONG_MAX \<Longrightarrow> (D :: 64 word) < C \<Longrightarrow> Suc (unat (D)) \<le> ULONG_MAX"
+  using foo3
+  by (simp add: less_eq_Suc_le) 
   
+
+
+
+lemma c_can_enq:
+  fixes rb :: "rb_C ptr"
+  shows 
+  "\<lbrace> \<lambda>s. rb_valid_c s rb  \<rbrace>
+   rb_can_enq_c_fun rb
+   \<lbrace> \<lambda> r s. r = (if rb_can_enq (rb_C_to_CleanQ_RB s rb) then 1 else 0) \<rbrace>!"
+  apply(subst rb_can_enq_c_fun_def)
+  apply(wp) 
+  unfolding rb_can_enq_def rb_full_def rb_C_to_CleanQ_RB_def 
+  apply(simp add:rb_valid_c_def)
+  using foo4 word_less_nat_alt by fastforce
+
+
+lemma c_rb_enq:
+  fixes rb :: "rb_C ptr" and b :: buffer_C
+  assumes full: "rb_can_enq_c_fun rb =  return (0)"
+  shows 
+  "\<lbrace> \<lambda>s. rb_valid_c s rb \<and> s0 = s  \<rbrace>
+   rb_enq_c_fun rb b
+   \<lbrace> \<lambda> r s. r \<noteq> 0 \<rbrace>!"
+   apply(subst rb_enq_c_fun_def)
+  apply(wp)
+   apply(auto)
+  apply(subst full)
+  apply(wp)
+  apply(simp)
+  done
+ 
+
   
+lemma c_rb_enq2:
+  fixes rb :: "rb_C ptr" and b :: buffer_C and s0 :: lifted_globals
+  assumes full: "rb_can_enq_c_fun rb =  return (0)"
+  shows "
+   \<lbrace> \<lambda>s. rb_valid_c s rb \<and> s0 = s  \<rbrace>
+   rb_enq_c_fun rb b
+   \<lbrace> \<lambda> r s. r \<noteq> 0 \<and> s = s0 \<rbrace>!"
+   apply(subst rb_enq_c_fun_def)
+   apply(auto)
+    apply(wp)
+   apply(simp)
+   apply(subst full)
+   apply(wp)
+  by(simp)
   
+lemma c_rb_enq3:
+  fixes rb :: "rb_C ptr" and b :: buffer_C and s0 :: lifted_globals
+  shows "
+   \<lbrace> \<lambda>s. rb_valid_c s rb \<and> s0 = s \<and> rb_can_enq_c_fun rb =  return (0)  \<rbrace>
+   rb_enq_c_fun rb b
+   \<lbrace> \<lambda> r s. r \<noteq> 0 \<and> s = s0 \<rbrace>!"
+  apply(subst rb_enq_c_fun_def)
+  apply(wp)
+  apply(auto)
+  apply(subst rb_can_enq_c_fun_def)
+  apply(wp)
+  apply(auto)
+  
+  by(simp)
+
+
+lemma "unat (C) \<le> ULONG_MAX \<Longrightarrow> D < C \<Longrightarrow> unat (D) < ULONG_MAX"
+
+
+  
+
+  
+
 
 
 
